\documentclass{article}
\usepackage[russian]{babel}
\usepackage{graphicx} % Required for inserting images

\title{СРВМ ДЗ 3}
\author{Dmitry Vasilkov}
\date{May 2023}

\begin{document}

\maketitle

\begin{center}
    \text{
Задание 329
}
\end{center}

\begin{center}
    \text{
$y''(x + 2)^5 = 1$
}
\end{center}

\begin{center}
    \text{
$u = x + 2$
}
\end{center}

\begin{center}
\text{$x = u - 2$}
\end{center}

\begin{center}
\text{
$u^5y'' = 1$
}
\end{center}

\begin{center}
\text{
$y'' = \frac{1}{u^5}$
}
\end{center}

\begin{center}
\text{
$y'' = \frac{d(y')}{du}$
}
\end{center}

\begin{center}
\text{
$\frac{d(y')}{du} = \frac{1}{u^5}$
}
\end{center}

\begin{center}
\text{
$\int d(y') = \int \frac{1}{u^5}du$
}
\end{center}

\begin{center}
\text{
$y' = C_1 - \frac{1}{4u^4}$
}
\end{center}

\begin{center}
\text{
$y'(u) = \frac{dy}{du}$
}
\end{center}

\begin{center}
\text{
$\frac{dy}{du} = C_1 - \frac{1}{4u^4}$
}
\end{center}

\begin{center}
\text{
$dy = (C_1 - \frac{1}{4u^4})du$
}
\end{center}

\begin{center}
\text{
$M(y)dy = N(u)du$
}
\end{center}

\begin{center}
\text{
$\int 1dy = \int C_1 - \frac{1}{4u^4}du$
}
\end{center}
\begin{center}
\text{
$y = \frac{12C_1u^4 + 1}{12u^3} + C_2$
}
\end{center}

\begin{center}
\text{
$u = x + 2$
}
\end{center}

\begin{center}
\text{
$y = \frac{1}{12(x + 2)^3} + C_1x + C_2 + 2C_1$
}
\end{center}

\begin{center}
\text{
$y = \frac{1}{12(x + 2)^3} + C_1x + C_2$\\\\
}\\\\
\end{center}

\begin{center}
\\\\
\text{
Задание 340
}
\end{center}

$$xy''' - y'' = 0$$

$$xy''' + y'' = (xy'')'$$

$$d(xy'' - 2y') = 0$$

$$xy'' - 2y' = C$$

$$xy'' - 2y' - C = 0$$

$$a = (ax)'$$

$$xy'' + y' = (xy')'$$

$$d(xy' - 3y - Cx) = 0$$

$$xy' - 3y - Cx = C_1$$

$$y' - \frac{3y}{x} - C = \frac{C_1}{x}$$

$$y' - \frac{3y}{x} = \frac{C_1}{x} + C$$

$$y' + a(x)y = b(x)$$

$$a = -\frac{3}{x}$$ 

$$b = \frac{C_1}{x} + C$$

$$y = uv$$

$$y' = uv' + u'v$$

$$uv' + u'v - \frac{3uv}{x} = \frac{C_1}{x} + C$$

$$u'v + u(v' - \frac{3v}{x}) = \frac{C_1}{x} + C$$

$$v' - \frac{3v}{x} = 0$$

$$v' = \frac{3v}{x}$$

$$v'(x) = \frac{dv}{dx}$$

$$\frac{dv}{dx} = \frac{3v}{x}$$

$$dv = \frac{3vdx}{x}$$

$$\frac{dv}{v} = \frac{3dx}{x}$$

$$M(v)dv = N(x)dx$$

$$\int \frac{1}{v}dv = \int \frac{3}{x}dx$$

$$ln(v) = 3ln(x)$$

$$e^{f_1} = e^{f_2}$$

$$v = x^3$$

$$u'v + u(v' - \frac{3v}{x}) = \frac{C_1}{x} + C$$

$$v = x^3$$

$$(v' - \frac{3v}{x}) = 0$$

$$u'x^3 = \frac{C_1}{x} + C$$

$$u' = \frac{Cx + C_1}{x^4}$$

$$u'(x) = \frac{du}{dx}$$

$$\frac{du}{dx} = \frac{Cx + C_1}{x^4}$$

$$du = \frac{(Cx + C_1)dx}{x^4}$$

$$M(u)du = N(x)dx$$

$$\int 1 du = \int \frac{Cx + C_1}{x^4}dx$$

$$u = C_2 - \frac{3Cx + 2C_1}{6x^3}$$

$$u = -\frac{C}{2x^2} - \frac{C_1}{3x^3} + C_2$$

$$u = \frac{y}{v}$$

$$v = x^3$$

$$y = \frac{6C_2x^3 - 3Cx - 2C_1}{6}$$

$$y = C_2x^3 + Cx + C_1$$

\begin{center}
\text{
Задание 345
}
\end{center}
$$y'' = \sqrt{
y' + 1
}$$

$$F(y, y', ..., y^{(n)}) = 0$$

$$y' = u(y)$$

$$y' = u$$

$$y'' = uu'$$

$$uu' = \sqrt{
u  + 1
}$$

$$u'(y) = \frac{du}{dy}$$

$$\frac{udu}{dy} = \sqrt{
u + 1
}$$

$$udu = \sqrt{
u + 1
}dy$$

$$\frac{udu}{\sqrt{u + 1}} = dy$$

$$M(u)du = N(y)dy$$

$$\int \frac{u}{\sqrt{u + 1}}du = \int 1dy$$

$$\frac{2u\sqrt{u + 1}}{3} - \frac{4\sqrt{u + 1}}{3} = y + C$$

$$\frac{2u\sqrt{u + 1}}{3} - \frac{4\sqrt{u + 1}}{3} = y + C, u = -1$$

$$u = y'$$

$$\frac{2y'\sqrt{y' + 1}}{3} - \frac{4\sqrt{y' + 1}}{3} = y + C$$

$$2y'\sqrt{y' + 1} - 4\sqrt{y' + 1} = 3y + 3C$$

$$F(x, y, y') = 0$$

$$y = f(x, y')$$

$$p = y'$$

$$p = y' = \frac{dy}{dx}$$

$$dy = pdx$$

$$y = \frac{2p\sqrt{p + 1}}{3} - \frac{4\sqrt{p + 1}}{3} - C$$

$$dy = \frac{pdp}{\sqrt{p + 1}}$$

$$dy = pdx$$

$$pdx = \frac{pdp}{\sqrt{p + 1}}$$

$$dx = \frac{dp}{\sqrt{p + 1}}$$

$$M(x)dx = N(p)dp$$

$$\int 1 dx = \int \frac{1}{\sqrt{p + 1}}dp$$

$$x = 2 \sqrt{p + 1} + C_1$$

$$p = \frac{x^2 - 2C_1x + C_1^2-4}{4}$$

$$y = \frac{2p\sqrt{p + 1}}{3} - \frac{4\sqrt{p + 1}}{3} - C$$

$$y = \frac{(x^2 - 2C_1x + C_1^2 - 12) \sqrt{x^2 - 2C_1x + C_1^2} - 12C}{12}$$

$$y = \frac{x^3}{12} - \frac{C_1x^2}{4} + \frac{C_1^2x}{4} - x + C$$

\end{document}
